Improve custom literals

src/Solver/Solvers.dfy
@@ -6,29 +6,37 @@ module Solvers {
   import opened DeclarationMarkers
 
   export
-    reveals SolverState, ProofResult
+    reveals SolverState, ProofResult, StackItem, SolverState.Evolves
     provides SolverState.Repr, SolverState.Valid
-    provides SolverState.stack, SolverState.declarations
+    provides SolverState.stack, SolverState.declarations, SolverState.additionalDeclaredNames
     reveals SolverState.IsTopMemo
     provides SolverState.Push, SolverState.Pop
-    provides SolverState.DeclareType, SolverState.AddDeclarationMarker, SolverState.DeclareSymbol, SolverState.AddAssumption, SolverState.Prove
+    provides SolverState.DeclareType, SolverState.AddDeclarationMarker, SolverState.DeclareSymbol, SolverState.DeclareAdditionalName
+    provides SolverState.AddAssumption, SolverState.Prove
     provides Smt, Basics, SolverExpr, DeclarationMarkers
 
   datatype ProofResult =
     | Proved
     | Unproved(reason: string)
+
+  datatype StackItem<Memo> = StackItem(memo: Memo, decls: set<DeclarationMarker>, names: set<string>)
   
   /// This solver state can backtrack, however, it cannot spawn new SMT instances.
   /// The solver state includes a stack of (memo, marker set) pairs, which allows the solver
   /// to be shared (in a sequential fashion) among several clients. The clients then update
   /// the stack and marker set to keep track of what has been given to the underlying SMT solver.
+  ///
+  /// Markers are typically of the type DeclarationMarker. For situations where it's awkward for
+  /// the client to create new DeclarationMarkers, there is also a set of strings that can be used
+  /// instead of or in addition to the set of DeclarationMarker.
   class SolverState<Memo(==)> {
     ghost const Repr: set<object>
 
     const smtEngine: Smt.SolverEngine
-    var stack: List<(Memo, set<DeclarationMarker>)>
+    var stack: List<StackItem<Memo>>
 
     var declarations: set<DeclarationMarker>
+    var additionalDeclaredNames: set<string>
 
     constructor (smtEngine: Smt.SolverEngine)
       requires smtEngine.Valid() && smtEngine.CommandStacks() == Cons(Nil, Nil)
@@ -37,6 +45,7 @@ module Solvers {
       this.smtEngine := smtEngine;
       this.stack := Nil;
       this.declarations := {};
+      this.additionalDeclaredNames := {};
       this.Repr := {this, smtEngine, smtEngine.process};
     }
 
@@ -52,37 +61,49 @@ module Solvers {
       && stack.Length() + 1 == smtEngine.CommandStacks().Length()
     }
 
+    twostate predicate Evolves()
+      reads this
+    {
+      && old(stack) == stack
+      && old(declarations) <= declarations
+      && old(additionalDeclaredNames) <= additionalDeclaredNames
+    }
+
     predicate IsTopMemo(m: Memo)
       reads this
     {
-      stack.Cons? && stack.head.0 == m
+      stack.Cons? && stack.head.memo == m
     }
 
     method Push(memo: Memo)
       requires Valid()
       modifies Repr
-      ensures Valid() && stack == Cons((memo, declarations), old(stack)) && declarations == old(declarations)
+      ensures Valid() && stack == Cons(StackItem(memo, declarations, additionalDeclaredNames), old(stack))
+      ensures declarations == old(declarations) && additionalDeclaredNames == old(additionalDeclaredNames)
     {
       smtEngine.Push();
-      stack := Cons((memo, declarations), stack);
+      stack := Cons(StackItem(memo, declarations, additionalDeclaredNames), stack);
     }
 
     method Pop()
       requires Valid() && stack.Cons?
       modifies Repr
-      ensures Valid() && stack == old(stack).tail && declarations == old(stack).head.1
+      ensures Valid() && stack == old(stack).tail
+      ensures declarations == old(stack).head.decls && additionalDeclaredNames == old(stack).head.names
     {
       smtEngine.CommandStacks().AboutDoubleCons();
       smtEngine.Pop();
-      var (_, decls) := stack.head;
+      var StackItem(_, decls, names) := stack.head;
       stack := stack.tail;
       declarations := decls;
+      additionalDeclaredNames := names;
     }
 
     method AddAssumption(expr: SExpr)
       requires Valid()
       modifies Repr
-      ensures Valid() && stack == old(stack) && declarations == old(declarations)
+      ensures Valid() && stack == old(stack)
+      ensures declarations == old(declarations) && additionalDeclaredNames == old(additionalDeclaredNames)
     {
       smtEngine.Assume(expr.ToString());
     }
@@ -90,7 +111,8 @@ module Solvers {
     method DeclareType(decl: STypeDecl, marker: DeclarationMarker)
       requires Valid()
       modifies Repr
-      ensures Valid() && stack == old(stack) && declarations == old(declarations) + {marker}
+      ensures Valid() && stack == old(stack)
+      ensures declarations == old(declarations) + {marker} && additionalDeclaredNames == old(additionalDeclaredNames)
     {
       smtEngine.DeclareSort(decl.name);
       declarations := declarations + {marker};
@@ -99,7 +121,8 @@ module Solvers {
     method AddDeclarationMarker(marker: DeclarationMarker)
       requires Valid()
       modifies Repr
-      ensures Valid() && stack == old(stack) && declarations == old(declarations) + {marker}
+      ensures Valid() && stack == old(stack)
+      ensures declarations == old(declarations) + {marker} && additionalDeclaredNames == old(additionalDeclaredNames)
     {
       declarations := declarations + {marker};
     }
@@ -107,16 +130,28 @@ module Solvers {
     method DeclareSymbol(decl: STypedDeclaration, marker: DeclarationMarker)
       requires Valid()
       modifies Repr
-      ensures Valid() && stack == old(stack) && declarations == old(declarations) + {marker}
+      ensures Valid() && stack == old(stack)
+      ensures declarations == old(declarations) + {marker} && additionalDeclaredNames == old(additionalDeclaredNames)
     {
       DeclareSymbolByName(decl.name, SType.TypesToSExpr(decl.inputTypes), decl.typ.ToSExpr());
       declarations := declarations + {marker};
     }
 
+    method DeclareAdditionalName(decl: STypedDeclaration, namedMarker: string)
+      requires Valid()
+      modifies Repr
+      ensures Valid() && stack == old(stack)
+      ensures declarations == old(declarations) && additionalDeclaredNames == old(additionalDeclaredNames) + {namedMarker}
+    {
+      DeclareSymbolByName(decl.name, SType.TypesToSExpr(decl.inputTypes), decl.typ.ToSExpr());
+      additionalDeclaredNames := additionalDeclaredNames + {namedMarker};
+    }
+
     method DeclareSymbolByName(name: string, inputTpe: SExpr, outputTpe: SExpr)
       requires Valid()
       modifies Repr
-      ensures Valid() && stack == old(stack) && declarations == old(declarations)
+      ensures Valid() && stack == old(stack)
+      ensures declarations == old(declarations) && additionalDeclaredNames == old(additionalDeclaredNames)
     {
       smtEngine.DeclareFunction(name, inputTpe.ToString(), outputTpe.ToString());
     }
@@ -124,7 +159,8 @@ module Solvers {
     method Prove(expr: SExpr) returns (result: ProofResult)
       requires Valid()
       modifies Repr
-      ensures Valid() && stack == old(stack) && declarations == old(declarations)
+      ensures Valid() && stack == old(stack)
+      ensures declarations == old(declarations) && additionalDeclaredNames == old(additionalDeclaredNames)
     {
       smtEngine.Push();
       smtEngine.Assume(SExpr.Negation(expr).ToString());
